src/Rewriter/Passes/Arith.v
@@ -22,6 +22,479 @@ Module Compilers.
       Definition VerifiedRewriterArith : VerifiedRewriter_with_args false false true (arith_rewrite_rules_proofs max_const_val).
       Proof using All. make_rewriter. Defined.
 
+      (*
+        Trying to add the rule
+          (Z.to_nat (1 + ((Z.of_nat i + 1)/2 - 1) - Z.of_nat (i - (n - 1))%nat)%Z) =
+          (Z.to_nat (1 + ((Z.of_nat i + 1)/2 - 1) - Z.of_nat (i - (n - 1))%nat)%Z))
+        causes make_rewriter to fail with the message:
+
+Error:
+In environment
+max_const_val : Z
+H : forall i n : nat,
+    Z.to_nat (1 + ((Z.of_nat i + 1) / 2 - 1) - Z.of_nat (i - (n - 1))) =
+    Z.to_nat (1 + ((Z.of_nat i + 1) / 2 - 1) - Z.of_nat (i - (n - 1)))
+v1 : RewriteRules.Compile.value' false
+       (type.base (base.type.type_base Compilers.nat))
+v2 : Compilers.base_interp Compilers.nat
+H0 : expr.interp_related (@Compilers.ident_interp) v1 v2
+v0 : RewriteRules.Compile.value' false
+       (type.base (base.type.type_base Compilers.nat))
+v3 : Compilers.base_interp Compilers.nat
+H1 : expr.interp_related (@Compilers.ident_interp) v0 v3
+v4 : RewriteRules.Compile.value' false
+       (type.base (base.type.type_base Compilers.nat))
+v5 : Compilers.base_interp Compilers.nat
+H2 : expr.interp_related (@Compilers.ident_interp) v4 v5
+Heqb2 : (1 =? 1) = true
+Heqb1_2 : (1 =? 1)%Z = true
+Heqb1_1_2 : (2 =? 2)%Z = true
+Heqb1_1_1_1, Heqb1_1_1_2 : (1 =? 1)%Z = true
+Unable to unify "v3" with "v2".
+       *)
+
+
+      
+
+      (* Trying to add the rule
+           (forall n x y, ident_adk_mul n x y = adk_mul n x y)
+         causes make_rewriter to fail with the message:
+
+============================
+WARNING: UNSOLVED GOAL:
+max_const_val : Z
+v1 : (API.expr (type.base (base.type.type_base Compilers.nat)))
+v2 : nat
+H0 :
+(expr.interp_related_gen (@Compilers.ident_interp)
+   (@type.related (Language.Compilers.base.type Compilers.base)
+      (Language.Compilers.base.interp Compilers.base_interp)
+      (fun t : Language.Compilers.base.type Compilers.base => eq)) v1 v2)
+v0 :
+(API.expr (type.base (base.type.list (base.type.type_base Compilers.Z))))
+v3 : (list Z)
+H1 :
+(expr.interp_related_gen (@Compilers.ident_interp)
+   (@type.related (Language.Compilers.base.type Compilers.base)
+      (Language.Compilers.base.interp Compilers.base_interp)
+      (fun t : Language.Compilers.base.type Compilers.base => eq)) v0 v3)
+v4 :
+(API.expr (type.base (base.type.list (base.type.type_base Compilers.Z))))
+v5 : (list Z)
+H2 :
+(expr.interp_related_gen (@Compilers.ident_interp)
+   (@type.related (Language.Compilers.base.type Compilers.base)
+      (Language.Compilers.base.interp Compilers.base_interp)
+      (fun t : Language.Compilers.base.type Compilers.base => eq)) v4 v5)
+x1 :
+(RewriteRules.Compile.value' false
+   (type.base (base.type.type_base Compilers.nat)))
+x2 : (API.interp_type (type.base (base.type.type_base Compilers.nat)))
+H :
+(ProofsCommon.Compilers.RewriteRules.Compile.value_interp_related
+   (@Compilers.ident_interp) x1 x2)
+x0 :
+(RewriteRules.Compile.value' false
+   (type.base (base.type.list (base.type.type_base Compilers.Z))))
+x3 :
+(API.interp_type
+   (type.base (base.type.list (base.type.type_base Compilers.Z))))
+H3 :
+(ProofsCommon.Compilers.RewriteRules.Compile.value_interp_related
+   (@Compilers.ident_interp) x0 x3)
+x4 :
+(RewriteRules.Compile.value' false
+   (type.base (base.type.list (base.type.type_base Compilers.Z))))
+x5 :
+(API.interp_type
+   (type.base (base.type.list (base.type.type_base Compilers.Z))))
+H4 :
+(ProofsCommon.Compilers.RewriteRules.Compile.value_interp_related
+   (@Compilers.ident_interp) x4 x5)
+============================
+(expr.interp_related_gen (@Compilers.ident_interp)
+   (fun t : API.type =>
+    ProofsCommon.Compilers.RewriteRules.Compile.value_interp_related
+      (@Compilers.ident_interp))
+   (expr_let v := (λ (v : API.expr
+                            (type.base (base.type.type_base Compilers.nat)))
+                   (v0 : API.expr
+                           (type.base
+                              (base.type.list
+                                 (base.type.type_base Compilers.Z))))
+                   (v1 : API.expr
+                           (type.base (base.type.type_base Compilers.Z))),
+                   #Compilers.ident_List_nth_default @ $$v1 @ $$v0 @ $$v) @
+                  (#Compilers.ident_Nat_sub @ $$x1 @ ###1) @ $$x0 @ ###0%Z *
+                  (λ (v : API.expr
+                            (type.base (base.type.type_base Compilers.nat)))
+                   (v0 : API.expr
+                           (type.base
+                              (base.type.list
+                                 (base.type.type_base Compilers.Z))))
+                   (v1 : API.expr
+                           (type.base (base.type.type_base Compilers.Z))),
+                   #Compilers.ident_List_nth_default @ $$v1 @ $$v0 @ $$v) @
+                  (#Compilers.ident_Nat_sub @ $$x1 @ ###1) @ $$x4 @ ###0%Z in
+    (λ v0 : API.expr
+              (type.base (base.type.list (base.type.type_base Compilers.Z))),
+     #Compilers.ident_list_rect_arrow @
+     (λ v1 : API.expr
+               (type.base (base.type.list (base.type.type_base Compilers.Z))),
+      (λ (v2 : API.expr (type.base (base.type.type_base Compilers.nat)))
+       (v3 v4 v5
+        v6 : API.expr
+               (type.base (base.type.list (base.type.type_base Compilers.Z)))),
+       #Compilers.ident_List_map @
+       ((λ (v7 : API.expr (type.base (base.type.type_base Compilers.nat)))
+         (v8 v9 v10
+          v11 : API.expr
+                  (type.base
+                     (base.type.list (base.type.type_base Compilers.Z))))
+         (v12 : API.expr (type.base (base.type.type_base Compilers.nat))),
+         #Compilers.ident_List_fold_right @ #Compilers.ident_Z_add @ ###0%Z @
+         (#Compilers.ident_List_map @
+          (λ v13 : API.expr (type.base (base.type.type_base Compilers.nat)),
+           ((λ (v14 : API.expr
+                        (type.base (base.type.type_base Compilers.nat)))
+             (v15 : API.expr
+                      (type.base
+                         (base.type.list (base.type.type_base Compilers.Z))))
+             (v16 : API.expr (type.base (base.type.type_base Compilers.Z))),
+             #Compilers.ident_List_nth_default @ $$v16 @ $$v15 @ $$v14) @
+            $$v13 @ $$v8 @ ###0%Z -
+            (λ (v14 : API.expr
+                        (type.base (base.type.type_base Compilers.nat)))
+             (v15 : API.expr
+                      (type.base
+                         (base.type.list (base.type.type_base Compilers.Z))))
+             (v16 : API.expr (type.base (base.type.type_base Compilers.Z))),
+             #Compilers.ident_List_nth_default @ $$v16 @ $$v15 @ $$v14) @
+            (#Compilers.ident_Nat_sub @ $$v12 @ $$v13) @ $$v8 @ ###0%Z) *
+           ((λ (v14 : API.expr
+                        (type.base (base.type.type_base Compilers.nat)))
+             (v15 : API.expr
+                      (type.base
+                         (base.type.list (base.type.type_base Compilers.Z))))
+             (v16 : API.expr (type.base (base.type.type_base Compilers.Z))),
+             #Compilers.ident_List_nth_default @ $$v16 @ $$v15 @ $$v14) @
+            (#Compilers.ident_Nat_sub @ $$v12 @ $$v13) @ $$v9 @ ###0%Z -
+            (λ (v14 : API.expr
+                        (type.base (base.type.type_base Compilers.nat)))
+             (v15 : API.expr
+                      (type.base
+                         (base.type.list (base.type.type_base Compilers.Z))))
+             (v16 : API.expr (type.base (base.type.type_base Compilers.Z))),
+             #Compilers.ident_List_nth_default @ $$v16 @ $$v15 @ $$v14) @
+            $$v13 @ $$v9 @ ###0%Z)) @
+          (#Compilers.ident_List_seq @
+           (#Compilers.ident_Nat_sub @ $$v12 @
+            (#Compilers.ident_Nat_sub @ $$v7 @ ###1)) @
+           (#Compilers.ident_Z_to_nat @
+            (###1%Z +
+             ((#Compilers.ident_Z_of_nat @ $$v12 + ###1%Z) / ###2%Z - ###1%Z) -
+             #Compilers.ident_Z_of_nat @
+             (#Compilers.ident_Nat_sub @ $$v12 @
+              (#Compilers.ident_Nat_sub @ $$v7 @ ###1)))))) +
+         #Compilers.ident_bool_rect @
+         (λ _ : API.expr (type.base ()),
+          (λ (v14 : API.expr (type.base (base.type.type_base Compilers.nat)))
+           (v15 : API.expr
+                    (type.base
+                       (base.type.list (base.type.type_base Compilers.Z))))
+           (v16 : API.expr (type.base (base.type.type_base Compilers.Z))),
+           #Compilers.ident_List_nth_default @ $$v16 @ $$v15 @ $$v14) @
+          (#Compilers.ident_Nat_sub @ $$v7 @ ###1) @ $$v10 @ ###0%Z) @
+         (λ _ : API.expr (type.base ()),
+          (λ (v14 : API.expr (type.base (base.type.type_base Compilers.nat)))
+           (v15 : API.expr
+                    (type.base
+                       (base.type.list (base.type.type_base Compilers.Z))))
+           (v16 : API.expr (type.base (base.type.type_base Compilers.Z))),
+           #Compilers.ident_List_nth_default @ $$v16 @ $$v15 @ $$v14) @ $$v12 @
+          $$v11 @ ###0%Z -
+          #Compilers.ident_bool_rect @ (λ _ : API.expr (type.base ()),
+                                        ###0%Z) @
+          (λ _ : API.expr (type.base ()),
+           (λ (v15 : API.expr (type.base (base.type.type_base Compilers.nat)))
+            (v16 : API.expr
+                     (type.base
+                        (base.type.list (base.type.type_base Compilers.Z))))
+            (v17 : API.expr (type.base (base.type.type_base Compilers.Z))),
+            #Compilers.ident_List_nth_default @ $$v17 @ $$v16 @ $$v15) @
+           (#Compilers.ident_Nat_sub @ $$v12 @ $$v7) @ $$v11 @ ###0%Z) @
+          (#Compilers.ident_Nat_ltb @ $$v12 @ $$v7)) @
+         (#Compilers.ident_Nat_eqb @ $$v12 @
+          (#Compilers.ident_Nat_sub @
+           (#Compilers.ident_Nat_mul @ ###2 @ $$v7) @ ###2))) @ $$v2 @ $$v3 @
+        $$v4 @ $$v5 @ $$v6) @
+       (#Compilers.ident_List_seq @ ###0 @
+        (#Compilers.ident_Nat_sub @ (#Compilers.ident_Nat_mul @ ###2 @ $$v2) @
+         ###1))) @ $$x1 @ $$x0 @ $$x4 @ $$v0 @
+      (#Compilers.ident_List_rev @ $$v1)) @
+     (λ (v1 : API.expr (type.base (base.type.type_base Compilers.Z)))
+      (_ : API.expr
+             (type.base (base.type.list (base.type.type_base Compilers.Z))))
+      (v3 : API.expr
+              (type.base (base.type.list (base.type.type_base Compilers.Z))) ->
+            UnderLets.UnderLets (Language.Compilers.base.type Compilers.base)
+              IdentifiersBasicGENERATED.Compilers.ident API.interp_type
+              (API.expr
+                 (type.base
+                    (base.type.list (base.type.type_base Compilers.Z)))))
+      (v4 : API.expr
+              (type.base (base.type.list (base.type.type_base Compilers.Z)))),
+      expr_let v5 := (λ (v5 : API.expr
+                                (type.base
+                                   (base.type.type_base Compilers.nat)))
+                      (v6 : API.expr
+                              (type.base
+                                 (base.type.list
+                                    (base.type.type_base Compilers.Z))))
+                      (v7 : API.expr
+                              (type.base (base.type.type_base Compilers.Z))),
+                      #Compilers.ident_List_nth_default @ $$v7 @ $$v6 @ $$v5) @
+                     ###0 @ $$v4 @ ###0%Z + $$v1 in
+      $$v3 @ ($$v5 :: $$v4)) @ $$v0 @ []) @
+    (#Compilers.ident_List_map @
+     (λ v0 : API.expr (type.base (base.type.type_base Compilers.nat)),
+      (λ (v1 : API.expr (type.base (base.type.type_base Compilers.nat)))
+       (v2 : API.expr
+               (type.base (base.type.list (base.type.type_base Compilers.Z))))
+       (v3 : API.expr (type.base (base.type.type_base Compilers.Z))),
+       #Compilers.ident_List_nth_default @ $$v3 @ $$v2 @ $$v1) @ $$v0 @ $$x0 @
+      ###0%Z *
+      (λ (v1 : API.expr (type.base (base.type.type_base Compilers.nat)))
+       (v2 : API.expr
+               (type.base (base.type.list (base.type.type_base Compilers.Z))))
+       (v3 : API.expr (type.base (base.type.type_base Compilers.Z))),
+       #Compilers.ident_List_nth_default @ $$v3 @ $$v2 @ $$v1) @ $$v0 @ $$x4 @
+      ###0%Z) @
+     (#Compilers.ident_List_seq @ ###0 @
+      (#Compilers.ident_Nat_sub @ $$x1 @ ###1)) ++
+     [$$v] ++
+     #Compilers.ident_List_repeat @ ###0%Z @
+     (#Compilers.ident_Nat_sub @ $$x1 @ ###1))) (ADK.adk_mul x2 x3 x5))
+============================
+Tactic call ran for 0.64 secs (0.639u,0.s) (success)
+WARNING: Remaining goal:
+max_const_val : Z
+v1 : (API.expr (type.base (base.type.type_base Compilers.nat)))
+v2 : nat
+H0 :
+(expr.interp_related_gen (@Compilers.ident_interp)
+   (@type.related (Language.Compilers.base.type Compilers.base)
+      (Language.Compilers.base.interp Compilers.base_interp)
+      (fun t : Language.Compilers.base.type Compilers.base => eq)) v1 v2)
+v0 :
+(API.expr (type.base (base.type.list (base.type.type_base Compilers.Z))))
+v3 : (list Z)
+H1 :
+(expr.interp_related_gen (@Compilers.ident_interp)
+   (@type.related (Language.Compilers.base.type Compilers.base)
+      (Language.Compilers.base.interp Compilers.base_interp)
+      (fun t : Language.Compilers.base.type Compilers.base => eq)) v0 v3)
+v4 :
+(API.expr (type.base (base.type.list (base.type.type_base Compilers.Z))))
+v5 : (list Z)
+H2 :
+(expr.interp_related_gen (@Compilers.ident_interp)
+   (@type.related (Language.Compilers.base.type Compilers.base)
+      (Language.Compilers.base.interp Compilers.base_interp)
+      (fun t : Language.Compilers.base.type Compilers.base => eq)) v4 v5)
+x1 :
+(RewriteRules.Compile.value' false
+   (type.base (base.type.type_base Compilers.nat)))
+x2 : (API.interp_type (type.base (base.type.type_base Compilers.nat)))
+H :
+(ProofsCommon.Compilers.RewriteRules.Compile.value_interp_related
+   (@Compilers.ident_interp) x1 x2)
+x0 :
+(RewriteRules.Compile.value' false
+   (type.base (base.type.list (base.type.type_base Compilers.Z))))
+x3 :
+(API.interp_type
+   (type.base (base.type.list (base.type.type_base Compilers.Z))))
+H3 :
+(ProofsCommon.Compilers.RewriteRules.Compile.value_interp_related
+   (@Compilers.ident_interp) x0 x3)
+x4 :
+(RewriteRules.Compile.value' false
+   (type.base (base.type.list (base.type.type_base Compilers.Z))))
+x5 :
+(API.interp_type
+   (type.base (base.type.list (base.type.type_base Compilers.Z))))
+H4 :
+(ProofsCommon.Compilers.RewriteRules.Compile.value_interp_related
+   (@Compilers.ident_interp) x4 x5)
+============================
+(expr.interp_related_gen (@Compilers.ident_interp)
+   (fun t : API.type =>
+    ProofsCommon.Compilers.RewriteRules.Compile.value_interp_related
+      (@Compilers.ident_interp))
+   (expr_let v := (λ (v : API.expr
+                            (type.base (base.type.type_base Compilers.nat)))
+                   (v0 : API.expr
+                           (type.base
+                              (base.type.list
+                                 (base.type.type_base Compilers.Z))))
+                   (v1 : API.expr
+                           (type.base (base.type.type_base Compilers.Z))),
+                   #Compilers.ident_List_nth_default @ $$v1 @ $$v0 @ $$v) @
+                  (#Compilers.ident_Nat_sub @ $$x1 @ ###1) @ $$x0 @ ###0%Z *
+                  (λ (v : API.expr
+                            (type.base (base.type.type_base Compilers.nat)))
+                   (v0 : API.expr
+                           (type.base
+                              (base.type.list
+                                 (base.type.type_base Compilers.Z))))
+                   (v1 : API.expr
+                           (type.base (base.type.type_base Compilers.Z))),
+                   #Compilers.ident_List_nth_default @ $$v1 @ $$v0 @ $$v) @
+                  (#Compilers.ident_Nat_sub @ $$x1 @ ###1) @ $$x4 @ ###0%Z in
+    (λ v0 : API.expr
+              (type.base (base.type.list (base.type.type_base Compilers.Z))),
+     #Compilers.ident_list_rect_arrow @
+     (λ v1 : API.expr
+               (type.base (base.type.list (base.type.type_base Compilers.Z))),
+      (λ (v2 : API.expr (type.base (base.type.type_base Compilers.nat)))
+       (v3 v4 v5
+        v6 : API.expr
+               (type.base (base.type.list (base.type.type_base Compilers.Z)))),
+       #Compilers.ident_List_map @
+       ((λ (v7 : API.expr (type.base (base.type.type_base Compilers.nat)))
+         (v8 v9 v10
+          v11 : API.expr
+                  (type.base
+                     (base.type.list (base.type.type_base Compilers.Z))))
+         (v12 : API.expr (type.base (base.type.type_base Compilers.nat))),
+         #Compilers.ident_List_fold_right @ #Compilers.ident_Z_add @ ###0%Z @
+         (#Compilers.ident_List_map @
+          (λ v13 : API.expr (type.base (base.type.type_base Compilers.nat)),
+           ((λ (v14 : API.expr
+                        (type.base (base.type.type_base Compilers.nat)))
+             (v15 : API.expr
+                      (type.base
+                         (base.type.list (base.type.type_base Compilers.Z))))
+             (v16 : API.expr (type.base (base.type.type_base Compilers.Z))),
+             #Compilers.ident_List_nth_default @ $$v16 @ $$v15 @ $$v14) @
+            $$v13 @ $$v8 @ ###0%Z -
+            (λ (v14 : API.expr
+                        (type.base (base.type.type_base Compilers.nat)))
+             (v15 : API.expr
+                      (type.base
+                         (base.type.list (base.type.type_base Compilers.Z))))
+             (v16 : API.expr (type.base (base.type.type_base Compilers.Z))),
+             #Compilers.ident_List_nth_default @ $$v16 @ $$v15 @ $$v14) @
+            (#Compilers.ident_Nat_sub @ $$v12 @ $$v13) @ $$v8 @ ###0%Z) *
+           ((λ (v14 : API.expr
+                        (type.base (base.type.type_base Compilers.nat)))
+             (v15 : API.expr
+                      (type.base
+                         (base.type.list (base.type.type_base Compilers.Z))))
+             (v16 : API.expr (type.base (base.type.type_base Compilers.Z))),
+             #Compilers.ident_List_nth_default @ $$v16 @ $$v15 @ $$v14) @
+            (#Compilers.ident_Nat_sub @ $$v12 @ $$v13) @ $$v9 @ ###0%Z -
+            (λ (v14 : API.expr
+                        (type.base (base.type.type_base Compilers.nat)))
+             (v15 : API.expr
+                      (type.base
+                         (base.type.list (base.type.type_base Compilers.Z))))
+             (v16 : API.expr (type.base (base.type.type_base Compilers.Z))),
+             #Compilers.ident_List_nth_default @ $$v16 @ $$v15 @ $$v14) @
+            $$v13 @ $$v9 @ ###0%Z)) @
+          (#Compilers.ident_List_seq @
+           (#Compilers.ident_Nat_sub @ $$v12 @
+            (#Compilers.ident_Nat_sub @ $$v7 @ ###1)) @
+           (#Compilers.ident_Z_to_nat @
+            (###1%Z +
+             ((#Compilers.ident_Z_of_nat @ $$v12 + ###1%Z) / ###2%Z - ###1%Z) -
+             #Compilers.ident_Z_of_nat @
+             (#Compilers.ident_Nat_sub @ $$v12 @
+              (#Compilers.ident_Nat_sub @ $$v7 @ ###1)))))) +
+         #Compilers.ident_bool_rect @
+         (λ _ : API.expr (type.base ()),
+          (λ (v14 : API.expr (type.base (base.type.type_base Compilers.nat)))
+           (v15 : API.expr
+                    (type.base
+                       (base.type.list (base.type.type_base Compilers.Z))))
+           (v16 : API.expr (type.base (base.type.type_base Compilers.Z))),
+           #Compilers.ident_List_nth_default @ $$v16 @ $$v15 @ $$v14) @
+          (#Compilers.ident_Nat_sub @ $$v7 @ ###1) @ $$v10 @ ###0%Z) @
+         (λ _ : API.expr (type.base ()),
+          (λ (v14 : API.expr (type.base (base.type.type_base Compilers.nat)))
+           (v15 : API.expr
+                    (type.base
+                       (base.type.list (base.type.type_base Compilers.Z))))
+           (v16 : API.expr (type.base (base.type.type_base Compilers.Z))),
+           #Compilers.ident_List_nth_default @ $$v16 @ $$v15 @ $$v14) @ $$v12 @
+          $$v11 @ ###0%Z -
+          #Compilers.ident_bool_rect @ (λ _ : API.expr (type.base ()),
+                                        ###0%Z) @
+          (λ _ : API.expr (type.base ()),
+           (λ (v15 : API.expr (type.base (base.type.type_base Compilers.nat)))
+            (v16 : API.expr
+                     (type.base
+                        (base.type.list (base.type.type_base Compilers.Z))))
+            (v17 : API.expr (type.base (base.type.type_base Compilers.Z))),
+            #Compilers.ident_List_nth_default @ $$v17 @ $$v16 @ $$v15) @
+           (#Compilers.ident_Nat_sub @ $$v12 @ $$v7) @ $$v11 @ ###0%Z) @
+          (#Compilers.ident_Nat_ltb @ $$v12 @ $$v7)) @
+         (#Compilers.ident_Nat_eqb @ $$v12 @
+          (#Compilers.ident_Nat_sub @
+           (#Compilers.ident_Nat_mul @ ###2 @ $$v7) @ ###2))) @ $$v2 @ $$v3 @
+        $$v4 @ $$v5 @ $$v6) @
+       (#Compilers.ident_List_seq @ ###0 @
+        (#Compilers.ident_Nat_sub @ (#Compilers.ident_Nat_mul @ ###2 @ $$v2) @
+         ###1))) @ $$x1 @ $$x0 @ $$x4 @ $$v0 @
+      (#Compilers.ident_List_rev @ $$v1)) @
+     (λ (v1 : API.expr (type.base (base.type.type_base Compilers.Z)))
+      (_ : API.expr
+             (type.base (base.type.list (base.type.type_base Compilers.Z))))
+      (v3 : API.expr
+              (type.base (base.type.list (base.type.type_base Compilers.Z))) ->
+            UnderLets.UnderLets (Language.Compilers.base.type Compilers.base)
+              IdentifiersBasicGENERATED.Compilers.ident API.interp_type
+              (API.expr
+                 (type.base
+                    (base.type.list (base.type.type_base Compilers.Z)))))
+      (v4 : API.expr
+              (type.base (base.type.list (base.type.type_base Compilers.Z)))),
+      expr_let v5 := (λ (v5 : API.expr
+                                (type.base
+                                   (base.type.type_base Compilers.nat)))
+                      (v6 : API.expr
+                              (type.base
+                                 (base.type.list
+                                    (base.type.type_base Compilers.Z))))
+                      (v7 : API.expr
+                              (type.base (base.type.type_base Compilers.Z))),
+                      #Compilers.ident_List_nth_default @ $$v7 @ $$v6 @ $$v5) @
+                     ###0 @ $$v4 @ ###0%Z + $$v1 in
+      $$v3 @ ($$v5 :: $$v4)) @ $$v0 @ []) @
+    (#Compilers.ident_List_map @
+     (λ v0 : API.expr (type.base (base.type.type_base Compilers.nat)),
+      (λ (v1 : API.expr (type.base (base.type.type_base Compilers.nat)))
+       (v2 : API.expr
+               (type.base (base.type.list (base.type.type_base Compilers.Z))))
+       (v3 : API.expr (type.base (base.type.type_base Compilers.Z))),
+       #Compilers.ident_List_nth_default @ $$v3 @ $$v2 @ $$v1) @ $$v0 @ $$x0 @
+      ###0%Z *
+      (λ (v1 : API.expr (type.base (base.type.type_base Compilers.nat)))
+       (v2 : API.expr
+               (type.base (base.type.list (base.type.type_base Compilers.Z))))
+       (v3 : API.expr (type.base (base.type.type_base Compilers.Z))),
+       #Compilers.ident_List_nth_default @ $$v3 @ $$v2 @ $$v1) @ $$v0 @ $$x4 @
+      ###0%Z) @
+     (#Compilers.ident_List_seq @ ###0 @
+      (#Compilers.ident_Nat_sub @ $$x1 @ ###1)) ++
+     [$$v] ++
+     #Compilers.ident_List_repeat @ ###0%Z @
+     (#Compilers.ident_Nat_sub @ $$x1 @ ###1))) (ADK.adk_mul x2 x3 x5))
+File "./src/Rewriter/Passes/Arith.v", line 23, characters 23-36:
+Error: Proof is not complete.
+       *)
+
       Definition default_opts := Eval hnf in @default_opts VerifiedRewriterArith.
       Let optsT := Eval hnf in optsT VerifiedRewriterArith.
 
